DynamoDbEncryption/runtimes/java/src/main/smithy-generated/software/amazon/cryptography/dynamoDbEncryption/ToNative.java
@@ -91,39 +91,6 @@ public class ToNative {
     return nativeBuilder.build();
   }
 
-  public static CompoundBeacon CompoundBeacon(
-      Dafny.Aws.Cryptography.DynamoDbEncryption.Types.CompoundBeacon dafnyValue) {
-    CompoundBeacon.Builder nativeBuilder = CompoundBeacon.builder();
-    nativeBuilder.name(software.amazon.dafny.conversion.ToNative.Simple.String(dafnyValue.dtor_name()));
-    nativeBuilder.split(software.amazon.dafny.conversion.ToNative.Simple.String(dafnyValue.dtor_split()));
-    if (dafnyValue.dtor_sensitive().is_Some()) {
-      nativeBuilder.sensitive(ToNative.SensitivePartsList(dafnyValue.dtor_sensitive().dtor_value()));
-    }
-    if (dafnyValue.dtor_nonSensitive().is_Some()) {
-      nativeBuilder.nonSensitive(ToNative.NonSensitivePartsList(dafnyValue.dtor_nonSensitive().dtor_value()));
-    }
-    if (dafnyValue.dtor_constructors().is_Some()) {
-      nativeBuilder.constructors(ToNative.ConstructorList(dafnyValue.dtor_constructors().dtor_value()));
-    }
-    return nativeBuilder.build();
-  }
-
-  public static DynamoDbEncryptionConfig DynamoDbEncryptionConfig(
-      Dafny.Aws.Cryptography.DynamoDbEncryption.Types.DynamoDbEncryptionConfig dafnyValue) {
-    DynamoDbEncryptionConfig.Builder nativeBuilder = DynamoDbEncryptionConfig.builder();
-    return nativeBuilder.build();
-  }
-
-  public static VirtualPart VirtualPart(
-      Dafny.Aws.Cryptography.DynamoDbEncryption.Types.VirtualPart dafnyValue) {
-    VirtualPart.Builder nativeBuilder = VirtualPart.builder();
-    nativeBuilder.loc(software.amazon.dafny.conversion.ToNative.Simple.String(dafnyValue.dtor_loc()));
-    if (dafnyValue.dtor_trans().is_Some()) {
-      nativeBuilder.trans(ToNative.VirtualTransformList(dafnyValue.dtor_trans().dtor_value()));
-    }
-    return nativeBuilder.build();
-  }
-
   public static SensitivePart SensitivePart(
       Dafny.Aws.Cryptography.DynamoDbEncryption.Types.SensitivePart dafnyValue) {
     SensitivePart.Builder nativeBuilder = SensitivePart.builder();
@@ -143,6 +110,13 @@ public class ToNative {
     return nativeBuilder.build();
   }
 
+  public static GetBranchKeyIdFromDdbKeyInput GetBranchKeyIdFromDdbKeyInput(
+      Dafny.Aws.Cryptography.DynamoDbEncryption.Types.GetBranchKeyIdFromDdbKeyInput dafnyValue) {
+    GetBranchKeyIdFromDdbKeyInput.Builder nativeBuilder = GetBranchKeyIdFromDdbKeyInput.builder();
+    nativeBuilder.ddbKey(Dafny.Com.Amazonaws.Dynamodb.ToNative.Key(dafnyValue.dtor_ddbKey()));
+    return nativeBuilder.build();
+  }
+
   public static GetSubstring GetSubstring(
       Dafny.Aws.Cryptography.DynamoDbEncryption.Types.GetSubstring dafnyValue) {
     GetSubstring.Builder nativeBuilder = GetSubstring.builder();
@@ -151,10 +125,35 @@ public class ToNative {
     return nativeBuilder.build();
   }
 
-  public static GetPrefix GetPrefix(
-      Dafny.Aws.Cryptography.DynamoDbEncryption.Types.GetPrefix dafnyValue) {
-    GetPrefix.Builder nativeBuilder = GetPrefix.builder();
-    nativeBuilder.length((dafnyValue.dtor_length()));
+  public static CompoundBeacon CompoundBeacon(
+      Dafny.Aws.Cryptography.DynamoDbEncryption.Types.CompoundBeacon dafnyValue) {
+    CompoundBeacon.Builder nativeBuilder = CompoundBeacon.builder();
+    nativeBuilder.name(software.amazon.dafny.conversion.ToNative.Simple.String(dafnyValue.dtor_name()));
+    nativeBuilder.split(software.amazon.dafny.conversion.ToNative.Simple.String(dafnyValue.dtor_split()));
+    if (dafnyValue.dtor_sensitive().is_Some()) {
+      nativeBuilder.sensitive(ToNative.SensitivePartsList(dafnyValue.dtor_sensitive().dtor_value()));
+    }
+    if (dafnyValue.dtor_nonSensitive().is_Some()) {
+      nativeBuilder.nonSensitive(ToNative.NonSensitivePartsList(dafnyValue.dtor_nonSensitive().dtor_value()));
+    }
+    if (dafnyValue.dtor_constructors().is_Some()) {
+      nativeBuilder.constructors(ToNative.ConstructorList(dafnyValue.dtor_constructors().dtor_value()));
+    }
+    return nativeBuilder.build();
+  }
+
+  public static Constructor Constructor(
+      Dafny.Aws.Cryptography.DynamoDbEncryption.Types.Constructor dafnyValue) {
+    Constructor.Builder nativeBuilder = Constructor.builder();
+    nativeBuilder.parts(ToNative.ConstructorPartList(dafnyValue.dtor_parts()));
+    return nativeBuilder.build();
+  }
+
+  public static ConstructorPart ConstructorPart(
+      Dafny.Aws.Cryptography.DynamoDbEncryption.Types.ConstructorPart dafnyValue) {
+    ConstructorPart.Builder nativeBuilder = ConstructorPart.builder();
+    nativeBuilder.name(software.amazon.dafny.conversion.ToNative.Simple.String(dafnyValue.dtor_name()));
+    nativeBuilder.required((dafnyValue.dtor_required()));
     return nativeBuilder.build();
   }
 
@@ -176,29 +175,32 @@ public class ToNative {
     return nativeBuilder.build();
   }
 
-  public static Constructor Constructor(
-      Dafny.Aws.Cryptography.DynamoDbEncryption.Types.Constructor dafnyValue) {
-    Constructor.Builder nativeBuilder = Constructor.builder();
-    nativeBuilder.parts(ToNative.ConstructorPartList(dafnyValue.dtor_parts()));
+  public static VirtualPart VirtualPart(
+      Dafny.Aws.Cryptography.DynamoDbEncryption.Types.VirtualPart dafnyValue) {
+    VirtualPart.Builder nativeBuilder = VirtualPart.builder();
+    nativeBuilder.loc(software.amazon.dafny.conversion.ToNative.Simple.String(dafnyValue.dtor_loc()));
+    if (dafnyValue.dtor_trans().is_Some()) {
+      nativeBuilder.trans(ToNative.VirtualTransformList(dafnyValue.dtor_trans().dtor_value()));
+    }
     return nativeBuilder.build();
   }
 
-  public static Upper Upper(Dafny.Aws.Cryptography.DynamoDbEncryption.Types.Upper dafnyValue) {
-    Upper.Builder nativeBuilder = Upper.builder();
+  public static DynamoDbEncryptionConfig DynamoDbEncryptionConfig(
+      Dafny.Aws.Cryptography.DynamoDbEncryption.Types.DynamoDbEncryptionConfig dafnyValue) {
+    DynamoDbEncryptionConfig.Builder nativeBuilder = DynamoDbEncryptionConfig.builder();
     return nativeBuilder.build();
   }
 
-  public static GetBranchKeyIdFromDdbKeyOutput GetBranchKeyIdFromDdbKeyOutput(
-      Dafny.Aws.Cryptography.DynamoDbEncryption.Types.GetBranchKeyIdFromDdbKeyOutput dafnyValue) {
-    GetBranchKeyIdFromDdbKeyOutput.Builder nativeBuilder = GetBranchKeyIdFromDdbKeyOutput.builder();
-    nativeBuilder.branchKeyId(software.amazon.dafny.conversion.ToNative.Simple.String(dafnyValue.dtor_branchKeyId()));
+  public static Insert Insert(Dafny.Aws.Cryptography.DynamoDbEncryption.Types.Insert dafnyValue) {
+    Insert.Builder nativeBuilder = Insert.builder();
+    nativeBuilder.literal(software.amazon.dafny.conversion.ToNative.Simple.String(dafnyValue.dtor_literal()));
     return nativeBuilder.build();
   }
 
-  public static GetBranchKeyIdFromDdbKeyInput GetBranchKeyIdFromDdbKeyInput(
-      Dafny.Aws.Cryptography.DynamoDbEncryption.Types.GetBranchKeyIdFromDdbKeyInput dafnyValue) {
-    GetBranchKeyIdFromDdbKeyInput.Builder nativeBuilder = GetBranchKeyIdFromDdbKeyInput.builder();
-    nativeBuilder.ddbKey(Dafny.Com.Amazonaws.Dynamodb.ToNative.Key(dafnyValue.dtor_ddbKey()));
+  public static GetPrefix GetPrefix(
+      Dafny.Aws.Cryptography.DynamoDbEncryption.Types.GetPrefix dafnyValue) {
+    GetPrefix.Builder nativeBuilder = GetPrefix.builder();
+    nativeBuilder.length((dafnyValue.dtor_length()));
     return nativeBuilder.build();
   }
 
@@ -209,11 +211,60 @@ public class ToNative {
     return nativeBuilder.build();
   }
 
-  public static ConstructorPart ConstructorPart(
-      Dafny.Aws.Cryptography.DynamoDbEncryption.Types.ConstructorPart dafnyValue) {
-    ConstructorPart.Builder nativeBuilder = ConstructorPart.builder();
-    nativeBuilder.name(software.amazon.dafny.conversion.ToNative.Simple.String(dafnyValue.dtor_name()));
-    nativeBuilder.required((dafnyValue.dtor_required()));
+  public static BeaconVersion BeaconVersion(
+      Dafny.Aws.Cryptography.DynamoDbEncryption.Types.BeaconVersion dafnyValue) {
+    BeaconVersion.Builder nativeBuilder = BeaconVersion.builder();
+    nativeBuilder.version((dafnyValue.dtor_version()));
+    nativeBuilder.keySource(ToNative.BeaconKeySource(dafnyValue.dtor_keySource()));
+    nativeBuilder.standardBeacons(ToNative.StandardBeaconList(dafnyValue.dtor_standardBeacons()));
+    if (dafnyValue.dtor_compoundBeacons().is_Some()) {
+      nativeBuilder.compoundBeacons(ToNative.CompoundBeaconList(dafnyValue.dtor_compoundBeacons().dtor_value()));
+    }
+    if (dafnyValue.dtor_virtualFields().is_Some()) {
+      nativeBuilder.virtualFields(ToNative.VirtualFieldList(dafnyValue.dtor_virtualFields().dtor_value()));
+    }
+    return nativeBuilder.build();
+  }
+
+  public static Lower Lower(Dafny.Aws.Cryptography.DynamoDbEncryption.Types.Lower dafnyValue) {
+    Lower.Builder nativeBuilder = Lower.builder();
+    return nativeBuilder.build();
+  }
+
+  public static SingleKeyStore SingleKeyStore(
+      Dafny.Aws.Cryptography.DynamoDbEncryption.Types.SingleKeyStore dafnyValue) {
+    SingleKeyStore.Builder nativeBuilder = SingleKeyStore.builder();
+    if (dafnyValue.dtor_keyStore().is_Some()) {
+      nativeBuilder.keyStore(software.amazon.cryptography.keyStore.ToNative.KeyStore(dafnyValue.dtor_keyStore().dtor_value()));
+    }
+    if (dafnyValue.dtor_keyId().is_Some()) {
+      nativeBuilder.keyId(software.amazon.dafny.conversion.ToNative.Simple.String(dafnyValue.dtor_keyId().dtor_value()));
+    }
+    if (dafnyValue.dtor_cacheTTL().is_Some()) {
+      nativeBuilder.cacheTTL((dafnyValue.dtor_cacheTTL().dtor_value()));
+    }
+    return nativeBuilder.build();
+  }
+
+  public static Upper Upper(Dafny.Aws.Cryptography.DynamoDbEncryption.Types.Upper dafnyValue) {
+    Upper.Builder nativeBuilder = Upper.builder();
+    return nativeBuilder.build();
+  }
+
+  public static GetSegment GetSegment(
+      Dafny.Aws.Cryptography.DynamoDbEncryption.Types.GetSegment dafnyValue) {
+    GetSegment.Builder nativeBuilder = GetSegment.builder();
+    nativeBuilder.split(software.amazon.dafny.conversion.ToNative.Simple.String(dafnyValue.dtor_split()));
+    nativeBuilder.index((dafnyValue.dtor_index()));
+    return nativeBuilder.build();
+  }
+
+  public static GetSegments GetSegments(
+      Dafny.Aws.Cryptography.DynamoDbEncryption.Types.GetSegments dafnyValue) {
+    GetSegments.Builder nativeBuilder = GetSegments.builder();
+    nativeBuilder.split(software.amazon.dafny.conversion.ToNative.Simple.String(dafnyValue.dtor_split()));
+    nativeBuilder.low((dafnyValue.dtor_low()));
+    nativeBuilder.high((dafnyValue.dtor_high()));
     return nativeBuilder.build();
   }
 
@@ -252,16 +303,21 @@ public class ToNative {
     return nativeBuilder.build();
   }
 
-  public static Lower Lower(Dafny.Aws.Cryptography.DynamoDbEncryption.Types.Lower dafnyValue) {
-    Lower.Builder nativeBuilder = Lower.builder();
+  public static NonSensitivePart NonSensitivePart(
+      Dafny.Aws.Cryptography.DynamoDbEncryption.Types.NonSensitivePart dafnyValue) {
+    NonSensitivePart.Builder nativeBuilder = NonSensitivePart.builder();
+    nativeBuilder.name(software.amazon.dafny.conversion.ToNative.Simple.String(dafnyValue.dtor_name()));
+    nativeBuilder.prefix(software.amazon.dafny.conversion.ToNative.Simple.String(dafnyValue.dtor_prefix()));
+    if (dafnyValue.dtor_loc().is_Some()) {
+      nativeBuilder.loc(software.amazon.dafny.conversion.ToNative.Simple.String(dafnyValue.dtor_loc().dtor_value()));
+    }
     return nativeBuilder.build();
   }
 
-  public static GetSegment GetSegment(
-      Dafny.Aws.Cryptography.DynamoDbEncryption.Types.GetSegment dafnyValue) {
-    GetSegment.Builder nativeBuilder = GetSegment.builder();
-    nativeBuilder.split(software.amazon.dafny.conversion.ToNative.Simple.String(dafnyValue.dtor_split()));
-    nativeBuilder.index((dafnyValue.dtor_index()));
+  public static GetBranchKeyIdFromDdbKeyOutput GetBranchKeyIdFromDdbKeyOutput(
+      Dafny.Aws.Cryptography.DynamoDbEncryption.Types.GetBranchKeyIdFromDdbKeyOutput dafnyValue) {
+    GetBranchKeyIdFromDdbKeyOutput.Builder nativeBuilder = GetBranchKeyIdFromDdbKeyOutput.builder();
+    nativeBuilder.branchKeyId(software.amazon.dafny.conversion.ToNative.Simple.String(dafnyValue.dtor_branchKeyId()));
     return nativeBuilder.build();
   }
 
@@ -272,76 +328,6 @@ public class ToNative {
     return nativeBuilder.build();
   }
 
-  public static BeaconVersion BeaconVersion(
-      Dafny.Aws.Cryptography.DynamoDbEncryption.Types.BeaconVersion dafnyValue) {
-    BeaconVersion.Builder nativeBuilder = BeaconVersion.builder();
-    nativeBuilder.version((dafnyValue.dtor_version()));
-    nativeBuilder.keySource(ToNative.BeaconKeySource(dafnyValue.dtor_keySource()));
-    if (dafnyValue.dtor_standardBeacons().is_Some()) {
-      nativeBuilder.standardBeacons(ToNative.StandardBeaconList(dafnyValue.dtor_standardBeacons().dtor_value()));
-    }
-    if (dafnyValue.dtor_compoundBeacons().is_Some()) {
-      nativeBuilder.compoundBeacons(ToNative.CompoundBeaconList(dafnyValue.dtor_compoundBeacons().dtor_value()));
-    }
-    if (dafnyValue.dtor_virtualFields().is_Some()) {
-      nativeBuilder.virtualFields(ToNative.VirtualFieldList(dafnyValue.dtor_virtualFields().dtor_value()));
-    }
-    return nativeBuilder.build();
-  }
-
-  public static SingleKeyStore SingleKeyStore(
-      Dafny.Aws.Cryptography.DynamoDbEncryption.Types.SingleKeyStore dafnyValue) {
-    SingleKeyStore.Builder nativeBuilder = SingleKeyStore.builder();
-    if (dafnyValue.dtor_keyStore().is_Some()) {
-      nativeBuilder.keyStore(software.amazon.cryptography.keyStore.ToNative.KeyStore(dafnyValue.dtor_keyStore().dtor_value()));
-    }
-    if (dafnyValue.dtor_keyId().is_Some()) {
-      nativeBuilder.keyId(software.amazon.dafny.conversion.ToNative.Simple.String(dafnyValue.dtor_keyId().dtor_value()));
-    }
-    if (dafnyValue.dtor_cacheTTL().is_Some()) {
-      nativeBuilder.cacheTTL((dafnyValue.dtor_cacheTTL().dtor_value()));
-    }
-    return nativeBuilder.build();
-  }
-
-  public static GetSegments GetSegments(
-      Dafny.Aws.Cryptography.DynamoDbEncryption.Types.GetSegments dafnyValue) {
-    GetSegments.Builder nativeBuilder = GetSegments.builder();
-    nativeBuilder.split(software.amazon.dafny.conversion.ToNative.Simple.String(dafnyValue.dtor_split()));
-    nativeBuilder.low((dafnyValue.dtor_low()));
-    nativeBuilder.high((dafnyValue.dtor_high()));
-    return nativeBuilder.build();
-  }
-
-  public static CreateDynamoDbEncryptionBranchKeyIdSupplierInput CreateDynamoDbEncryptionBranchKeyIdSupplierInput(
-      Dafny.Aws.Cryptography.DynamoDbEncryption.Types.CreateDynamoDbEncryptionBranchKeyIdSupplierInput dafnyValue) {
-    CreateDynamoDbEncryptionBranchKeyIdSupplierInput.Builder nativeBuilder = CreateDynamoDbEncryptionBranchKeyIdSupplierInput.builder();
-    nativeBuilder.ddbKeyBranchKeyIdSupplier(ToNative.DynamoDbKeyBranchKeyIdSupplier(dafnyValue.dtor_ddbKeyBranchKeyIdSupplier()));
-    return nativeBuilder.build();
-  }
-
-  public static VirtualField VirtualField(
-      Dafny.Aws.Cryptography.DynamoDbEncryption.Types.VirtualField dafnyValue) {
-    VirtualField.Builder nativeBuilder = VirtualField.builder();
-    nativeBuilder.name(software.amazon.dafny.conversion.ToNative.Simple.String(dafnyValue.dtor_name()));
-    nativeBuilder.parts(ToNative.VirtualPartList(dafnyValue.dtor_parts()));
-    return nativeBuilder.build();
-  }
-
-  public static Insert Insert(Dafny.Aws.Cryptography.DynamoDbEncryption.Types.Insert dafnyValue) {
-    Insert.Builder nativeBuilder = Insert.builder();
-    nativeBuilder.literal(software.amazon.dafny.conversion.ToNative.Simple.String(dafnyValue.dtor_literal()));
-    return nativeBuilder.build();
-  }
-
-  public static SearchConfig SearchConfig(
-      Dafny.Aws.Cryptography.DynamoDbEncryption.Types.SearchConfig dafnyValue) {
-    SearchConfig.Builder nativeBuilder = SearchConfig.builder();
-    nativeBuilder.versions(ToNative.BeaconVersionList(dafnyValue.dtor_versions()));
-    nativeBuilder.writeVersion((dafnyValue.dtor_writeVersion()));
-    return nativeBuilder.build();
-  }
-
   public static DynamoDbTablesEncryptionConfig DynamoDbTablesEncryptionConfig(
       Dafny.Aws.Cryptography.DynamoDbEncryption.Types.DynamoDbTablesEncryptionConfig dafnyValue) {
     DynamoDbTablesEncryptionConfig.Builder nativeBuilder = DynamoDbTablesEncryptionConfig.builder();
@@ -349,14 +335,10 @@ public class ToNative {
     return nativeBuilder.build();
   }
 
-  public static NonSensitivePart NonSensitivePart(
-      Dafny.Aws.Cryptography.DynamoDbEncryption.Types.NonSensitivePart dafnyValue) {
-    NonSensitivePart.Builder nativeBuilder = NonSensitivePart.builder();
-    nativeBuilder.name(software.amazon.dafny.conversion.ToNative.Simple.String(dafnyValue.dtor_name()));
-    nativeBuilder.prefix(software.amazon.dafny.conversion.ToNative.Simple.String(dafnyValue.dtor_prefix()));
-    if (dafnyValue.dtor_loc().is_Some()) {
-      nativeBuilder.loc(software.amazon.dafny.conversion.ToNative.Simple.String(dafnyValue.dtor_loc().dtor_value()));
-    }
+  public static CreateDynamoDbEncryptionBranchKeyIdSupplierInput CreateDynamoDbEncryptionBranchKeyIdSupplierInput(
+      Dafny.Aws.Cryptography.DynamoDbEncryption.Types.CreateDynamoDbEncryptionBranchKeyIdSupplierInput dafnyValue) {
+    CreateDynamoDbEncryptionBranchKeyIdSupplierInput.Builder nativeBuilder = CreateDynamoDbEncryptionBranchKeyIdSupplierInput.builder();
+    nativeBuilder.ddbKeyBranchKeyIdSupplier(ToNative.DynamoDbKeyBranchKeyIdSupplier(dafnyValue.dtor_ddbKeyBranchKeyIdSupplier()));
     return nativeBuilder.build();
   }
 
@@ -369,6 +351,22 @@ public class ToNative {
     if (dafnyValue.dtor_defaultAttributeFlag().is_Some()) {
       nativeBuilder.defaultAttributeFlag(software.amazon.cryptography.structuredEncryption.ToNative.CryptoAction(dafnyValue.dtor_defaultAttributeFlag().dtor_value()));
     }
+    return nativeBuilder.build();
+  }
+
+  public static SearchConfig SearchConfig(
+      Dafny.Aws.Cryptography.DynamoDbEncryption.Types.SearchConfig dafnyValue) {
+    SearchConfig.Builder nativeBuilder = SearchConfig.builder();
+    nativeBuilder.versions(ToNative.BeaconVersionList(dafnyValue.dtor_versions()));
+    nativeBuilder.writeVersion((dafnyValue.dtor_writeVersion()));
+    return nativeBuilder.build();
+  }
+
+  public static VirtualField VirtualField(
+      Dafny.Aws.Cryptography.DynamoDbEncryption.Types.VirtualField dafnyValue) {
+    VirtualField.Builder nativeBuilder = VirtualField.builder();
+    nativeBuilder.name(software.amazon.dafny.conversion.ToNative.Simple.String(dafnyValue.dtor_name()));
+    nativeBuilder.parts(ToNative.VirtualPartList(dafnyValue.dtor_parts()));
     return nativeBuilder.build();
   }
 
@@ -398,6 +396,18 @@ public class ToNative {
       return LegacyPolicy.FORBID_ENCRYPT_FORBID_DECRYPT;
     }
     throw new IllegalArgumentException("No entry of software.amazon.cryptography.dynamoDbEncryption.model.LegacyPolicy matches the input : " + dafnyValue);
+  }
+
+  public static BeaconKeySource BeaconKeySource(
+      Dafny.Aws.Cryptography.DynamoDbEncryption.Types.BeaconKeySource dafnyValue) {
+    BeaconKeySource.Builder nativeBuilder = BeaconKeySource.builder();
+    if (dafnyValue.is_single()) {
+      nativeBuilder.single(ToNative.SingleKeyStore(dafnyValue.dtor_single()));
+    }
+    if (dafnyValue.is_multi()) {
+      nativeBuilder.multi(ToNative.MultiKeyStore(dafnyValue.dtor_multi()));
+    }
+    return nativeBuilder.build();
   }
 
   public static VirtualTransform VirtualTransform(
@@ -430,30 +440,11 @@ public class ToNative {
     return nativeBuilder.build();
   }
 
-  public static BeaconKeySource BeaconKeySource(
-      Dafny.Aws.Cryptography.DynamoDbEncryption.Types.BeaconKeySource dafnyValue) {
-    BeaconKeySource.Builder nativeBuilder = BeaconKeySource.builder();
-    if (dafnyValue.is_single()) {
-      nativeBuilder.single(ToNative.SingleKeyStore(dafnyValue.dtor_single()));
-    }
-    if (dafnyValue.is_multi()) {
-      nativeBuilder.multi(ToNative.MultiKeyStore(dafnyValue.dtor_multi()));
-    }
-    return nativeBuilder.build();
-  }
-
-  public static List<NonSensitivePart> NonSensitivePartsList(
-      DafnySequence<? extends Dafny.Aws.Cryptography.DynamoDbEncryption.Types.NonSensitivePart> dafnyValue) {
+  public static List<ConstructorPart> ConstructorPartList(
+      DafnySequence<? extends Dafny.Aws.Cryptography.DynamoDbEncryption.Types.ConstructorPart> dafnyValue) {
     return software.amazon.dafny.conversion.ToNative.Aggregate.GenericToList(
         dafnyValue, 
-        software.amazon.cryptography.dynamoDbEncryption.ToNative::NonSensitivePart);
-  }
-
-  public static List<VirtualField> VirtualFieldList(
-      DafnySequence<? extends Dafny.Aws.Cryptography.DynamoDbEncryption.Types.VirtualField> dafnyValue) {
-    return software.amazon.dafny.conversion.ToNative.Aggregate.GenericToList(
-        dafnyValue, 
-        software.amazon.cryptography.dynamoDbEncryption.ToNative::VirtualField);
+        software.amazon.cryptography.dynamoDbEncryption.ToNative::ConstructorPart);
   }
 
   public static List<StandardBeacon> StandardBeaconList(
@@ -463,32 +454,18 @@ public class ToNative {
         software.amazon.cryptography.dynamoDbEncryption.ToNative::StandardBeacon);
   }
 
-  public static List<ConstructorPart> ConstructorPartList(
-      DafnySequence<? extends Dafny.Aws.Cryptography.DynamoDbEncryption.Types.ConstructorPart> dafnyValue) {
+  public static List<VirtualPart> VirtualPartList(
+      DafnySequence<? extends Dafny.Aws.Cryptography.DynamoDbEncryption.Types.VirtualPart> dafnyValue) {
     return software.amazon.dafny.conversion.ToNative.Aggregate.GenericToList(
         dafnyValue, 
-        software.amazon.cryptography.dynamoDbEncryption.ToNative::ConstructorPart);
+        software.amazon.cryptography.dynamoDbEncryption.ToNative::VirtualPart);
   }
 
-  public static List<BeaconVersion> BeaconVersionList(
-      DafnySequence<? extends Dafny.Aws.Cryptography.DynamoDbEncryption.Types.BeaconVersion> dafnyValue) {
+  public static List<NonSensitivePart> NonSensitivePartsList(
+      DafnySequence<? extends Dafny.Aws.Cryptography.DynamoDbEncryption.Types.NonSensitivePart> dafnyValue) {
     return software.amazon.dafny.conversion.ToNative.Aggregate.GenericToList(
         dafnyValue, 
-        software.amazon.cryptography.dynamoDbEncryption.ToNative::BeaconVersion);
-  }
-
-  public static List<Constructor> ConstructorList(
-      DafnySequence<? extends Dafny.Aws.Cryptography.DynamoDbEncryption.Types.Constructor> dafnyValue) {
-    return software.amazon.dafny.conversion.ToNative.Aggregate.GenericToList(
-        dafnyValue, 
-        software.amazon.cryptography.dynamoDbEncryption.ToNative::Constructor);
-  }
-
-  public static List<CompoundBeacon> CompoundBeaconList(
-      DafnySequence<? extends Dafny.Aws.Cryptography.DynamoDbEncryption.Types.CompoundBeacon> dafnyValue) {
-    return software.amazon.dafny.conversion.ToNative.Aggregate.GenericToList(
-        dafnyValue, 
-        software.amazon.cryptography.dynamoDbEncryption.ToNative::CompoundBeacon);
+        software.amazon.cryptography.dynamoDbEncryption.ToNative::NonSensitivePart);
   }
 
   public static List<VirtualTransform> VirtualTransformList(
@@ -498,6 +475,13 @@ public class ToNative {
         software.amazon.cryptography.dynamoDbEncryption.ToNative::VirtualTransform);
   }
 
+  public static List<Constructor> ConstructorList(
+      DafnySequence<? extends Dafny.Aws.Cryptography.DynamoDbEncryption.Types.Constructor> dafnyValue) {
+    return software.amazon.dafny.conversion.ToNative.Aggregate.GenericToList(
+        dafnyValue, 
+        software.amazon.cryptography.dynamoDbEncryption.ToNative::Constructor);
+  }
+
   public static List<SensitivePart> SensitivePartsList(
       DafnySequence<? extends Dafny.Aws.Cryptography.DynamoDbEncryption.Types.SensitivePart> dafnyValue) {
     return software.amazon.dafny.conversion.ToNative.Aggregate.GenericToList(
@@ -505,19 +489,25 @@ public class ToNative {
         software.amazon.cryptography.dynamoDbEncryption.ToNative::SensitivePart);
   }
 
-  public static List<VirtualPart> VirtualPartList(
-      DafnySequence<? extends Dafny.Aws.Cryptography.DynamoDbEncryption.Types.VirtualPart> dafnyValue) {
+  public static List<CompoundBeacon> CompoundBeaconList(
+      DafnySequence<? extends Dafny.Aws.Cryptography.DynamoDbEncryption.Types.CompoundBeacon> dafnyValue) {
     return software.amazon.dafny.conversion.ToNative.Aggregate.GenericToList(
         dafnyValue, 
-        software.amazon.cryptography.dynamoDbEncryption.ToNative::VirtualPart);
+        software.amazon.cryptography.dynamoDbEncryption.ToNative::CompoundBeacon);
   }
 
-  public static Map<String, DynamoDbTableEncryptionConfig> DynamoDbTableEncryptionConfigList(
-      DafnyMap<? extends DafnySequence<? extends Character>, ? extends Dafny.Aws.Cryptography.DynamoDbEncryption.Types.DynamoDbTableEncryptionConfig> dafnyValue) {
-    return software.amazon.dafny.conversion.ToNative.Aggregate.GenericToMap(
+  public static List<BeaconVersion> BeaconVersionList(
+      DafnySequence<? extends Dafny.Aws.Cryptography.DynamoDbEncryption.Types.BeaconVersion> dafnyValue) {
+    return software.amazon.dafny.conversion.ToNative.Aggregate.GenericToList(
         dafnyValue, 
-        software.amazon.dafny.conversion.ToNative.Simple::String, 
-        software.amazon.cryptography.dynamoDbEncryption.ToNative::DynamoDbTableEncryptionConfig);
+        software.amazon.cryptography.dynamoDbEncryption.ToNative::BeaconVersion);
+  }
+
+  public static List<VirtualField> VirtualFieldList(
+      DafnySequence<? extends Dafny.Aws.Cryptography.DynamoDbEncryption.Types.VirtualField> dafnyValue) {
+    return software.amazon.dafny.conversion.ToNative.Aggregate.GenericToList(
+        dafnyValue, 
+        software.amazon.cryptography.dynamoDbEncryption.ToNative::VirtualField);
   }
 
   public static Map<String, CryptoAction> AttributeActions(
@@ -528,13 +518,21 @@ public class ToNative {
         software.amazon.cryptography.structuredEncryption.ToNative::CryptoAction);
   }
 
-  public static LegacyDynamoDbEncryptor LegacyDynamoDbEncryptor(
-      ILegacyDynamoDbEncryptor dafnyValue) {
-    return LegacyDynamoDbEncryptor.wrap(dafnyValue);
+  public static Map<String, DynamoDbTableEncryptionConfig> DynamoDbTableEncryptionConfigList(
+      DafnyMap<? extends DafnySequence<? extends Character>, ? extends Dafny.Aws.Cryptography.DynamoDbEncryption.Types.DynamoDbTableEncryptionConfig> dafnyValue) {
+    return software.amazon.dafny.conversion.ToNative.Aggregate.GenericToMap(
+        dafnyValue, 
+        software.amazon.dafny.conversion.ToNative.Simple::String, 
+        software.amazon.cryptography.dynamoDbEncryption.ToNative::DynamoDbTableEncryptionConfig);
   }
 
   public static DynamoDbKeyBranchKeyIdSupplier DynamoDbKeyBranchKeyIdSupplier(
       IDynamoDbKeyBranchKeyIdSupplier dafnyValue) {
     return DynamoDbKeyBranchKeyIdSupplier.wrap(dafnyValue);
+  }
+
+  public static LegacyDynamoDbEncryptor LegacyDynamoDbEncryptor(
+      ILegacyDynamoDbEncryptor dafnyValue) {
+    return LegacyDynamoDbEncryptor.wrap(dafnyValue);
   }
 }
